Strata/DL/Lambda/LExprTypeSpec.lean
@@ -45,7 +45,7 @@ def LTy.open (x : TyIdentifier) (xty : LMonoTy) (ty : LTy) : LTy :=
   | .forAll vars lty =>
     if x ∈ vars then
       let S := [(x, xty)]
-      .forAll (vars.removeAll [x]) (LMonoTy.subst S lty)
+      .forAll (vars.removeAll [x]) (LMonoTy.subst [S] lty)
     else
       ty
 
@@ -165,7 +165,7 @@ example : LExpr.HasType { types := [[("x", t[∀a. %a])]]} esM[x] t[int] := by
   simp +ground at h_tvar
   simp [h_tvar] at h_tinst
   simp +ground at h_tinst
-  simp [Map.isEmpty, Bool.decEq] at h_tinst
+  simp [Maps.isEmpty, Bool.decEq] at h_tinst
   assumption
 
 example : LExpr.HasType { types := [[("m", t[∀a. %a → int])]]}
@@ -177,7 +177,7 @@ example : LExpr.HasType { types := [[("m", t[∀a. %a → int])]]}
   · apply LExpr.HasType.tvar
     simp +ground
   · simp +ground
-    simp [Map.isEmpty, Bool.decEq]
+    simp [Maps.isEmpty, Bool.decEq]
   done
 
 example : LExpr.HasType {} esM[λ %0] t[∀a. %a → %a] := by
